pulse/lib/pulse/core/PulseCore.IndirectionTheorySep.fst
@@ -24,7 +24,7 @@ let is_ghost_action =
 let lift_ghost_action m p = ()
 
 let update_ghost m1 m2 =
-  (I.reveal_istore (fst m2), {
+  (I.reveal_hogs (fst m2), {
     I.saved_credits = (snd m2).saved_credits;
     I.timeless_heap = PM.pulse_heap_sig.update_ghost (timeless_mem_of m1) (timeless_mem_of m2);
   })
@@ -46,11 +46,11 @@ let sep_laws = I.sep_laws
 let disjoint m1 m2 = I.disjoint_worlds m1 m2
 let join m1 m2 = I.join_worlds m1 m2
 
-let clear_except_istore i = (fst i, I.empty_rest)
+let clear_except_hogs i = (fst i, I.empty_rest)
 
 let join_refl i =
   PM.pulse_heap_sig.sep.join_empty (snd i).timeless_heap;
-  I.join_istore_refl (fst i)
+  I.join_hogs_refl (fst i)
 
 let disjoint_join_levels i0 i1 = ()
 
@@ -123,17 +123,17 @@ let iref = I.iref
 let deq_iref = fun x y -> reveal x = reveal y
 let lower_inames i = GhostSet.empty
 
-let istore_inames_ok e m = I.inames_ok e (fst m)
+let hogs_inames_ok e m = I.inames_ok e (fst m)
 
 let inames_ok_empty m = ()
 let inames_ok_union i j m =
   assert (I.inames_ok (FStar.GhostSet.union i j) (fst m) <==>
     I.inames_ok i (fst m) /\ I.inames_ok j (fst m))
 
-let istore_invariant ex i = I.istore_invariant ex (fst i)
+let hogs_invariant ex i = I.hogs_invariant ex (fst i)
 
 let inames_ok_update_timeless_mem m p ex = ()
-let istore_invariant_update_timeless_mem m p ex = ()
+let hogs_invariant_update_timeless_mem m p ex = ()
 
 let inv i p = I.inv i p
 
@@ -163,14 +163,14 @@ let equiv_star_congr p q r = I.equiv_star_congr p q r
 
 let intro_later p m = ()
 
-let istore_dom m = I.istore_dom (fst m)
+let hogs_dom m = I.hogs_dom (fst m)
 
 let pulse_ghost_action_refl m : Lemma (PM.is_ghost_action m m) [SMTPat (PM.is_ghost_action m m)] =
   PM.pulse_heap_sig.is_ghost_action_preorder ()
 
 let age_mem m =
   let m' = I.age1_ m in
-  GhostSet.lemma_equal_intro (istore_dom m) (istore_dom m'); assert istore_dom m == istore_dom m';
+  GhostSet.lemma_equal_intro (hogs_dom m) (hogs_dom m'); assert hogs_dom m == hogs_dom m';
   m'
 
 let age_level m = ()
@@ -209,13 +209,13 @@ let single_eq i : Lemma (single i == I.single i) [SMTPat (single i)] =
   assert_norm (single i == I.single i) // why???
 
 let mem_invariant_equiv e m i = 
-  I.istore_invariant_equiv e (fst m) i;
+  I.hogs_invariant_equiv e (fst m) i;
   sep_laws()
 
-let inames_ok_istore_dom e m = ()
+let inames_ok_hogs_dom e m = ()
 
 let inames_ok_update e m0 m1 =
-  assert forall i. GhostSet.mem i (istore_dom m0) <==> GhostSet.mem i (istore_dom m1)
+  assert forall i. GhostSet.mem i (hogs_dom m0) <==> GhostSet.mem i (hogs_dom m1)
 
 // let pulse_of (m: timeless_mem) : timeless_mem = m
 // let pulse_join_mem (m0: timeless_mem) (m1: timeless_mem { PM.pulse_heap_sig.sep.disjoint (pulse_of m0) (pulse_of m1) }) 
@@ -237,7 +237,7 @@ let mem_invariant_disjoint (e f:inames) (p0 p1:slprop) (m0 m1:mem) =
   sep_laws ();
   let p0' = (p0 `star` lift (PM.mem_invariant GhostSet.empty (timeless_mem_of m0))) in
   let p1' = (p1 `star` lift (PM.mem_invariant GhostSet.empty (timeless_mem_of m1))) in
-  I.istore_invariant_disjoint' e f p0' p1' m0 m1;
+  I.hogs_invariant_disjoint' e f p0' p1' m0 m1;
   let m = join_mem m0 m1 in
   let cm = m in
   let im = I.join_worlds m0 m1 in
@@ -250,14 +250,14 @@ let mem_invariant_age e m0 m1 =
   with _ . (
     let m10, m11 =
       split_mem (lift (PM.mem_invariant GhostSet.empty (timeless_mem_of m0)))
-                (istore_invariant e m0) m1
+                (hogs_invariant e m0) m1
     in
-    I.istore_invariant_age e (fst m0) (m11);
+    I.hogs_invariant_age e (fst m0) (m11);
     age_hereditary (lift (PM.mem_invariant GhostSet.empty (timeless_mem_of m0))) m10;
-    assert (interp (istore_invariant e (age_mem m0)) (age1 m11));
+    assert (interp (hogs_invariant e (age_mem m0)) (age1 m11));
     age_disjoint m10 m11;
     intro_star (lift (PM.mem_invariant GhostSet.empty (timeless_mem_of m0)))
-                (istore_invariant e (age_mem m0)) 
+                (hogs_invariant e (age_mem m0)) 
                 (age1 m10)
                 (age1 m11)
   )
@@ -279,7 +279,7 @@ let fresh_inv p m ctx =
   let m': mem = (I.fresh_inv p (fst m) i, I.empty_rest) in
   let _: squash (inv i p `star` mem_invariant (single i) m' == inv i p) =
     pm_mem_invariant_empty();
-    I.istore_single_invariant (level m) i p;
+    I.hogs_single_invariant (level m) i p;
     sep_laws () in
   Classical.forall_intro (PM.pulse_heap_sig.sep.join_empty);
   (| i, m' |)
