pulse/lib/pulse/core/PulseCore.IndirectionTheorySepImpl.fst
@@ -16,32 +16,32 @@ let timeless_mem : Type u#4 = PM.mem u#0
 let timeless_heap_sig : HS.heap_sig u#3 = PM.pulse_heap_sig
 
 [@@erasable]
-noeq type istore_val_ (x: Type u#4) =
+noeq type hogs_val_ (x: Type u#4) =
   | None
-  | Inv : x -> istore_val_ x
-  | Pred : x -> istore_val_ x
+  | Inv : x -> hogs_val_ x
+  | Pred : x -> hogs_val_ x
 
-let istore_val_le #t (x y: istore_val_ t) : prop =
+let hogs_val_le #t (x y: hogs_val_ t) : prop =
   match x, y with
   | None, _ -> True
   | Inv p, Inv q -> p == q
   | Pred p, Pred q -> p == q
   | _ -> False
 
-let map_istore_val #x #y (f: x->y) (v: istore_val_ x) : istore_val_ y =
+let map_hogs_val #x #y (f: x->y) (v: hogs_val_ x) : hogs_val_ y =
   match v with
   | None -> None
   | Pred p -> Pred (f p)
   | Inv p -> Inv (f p)
 
 [@@erasable]
-let invariants (x:Type u#4) : Type u#4 = address ^-> istore_val_ x
+let invariants (x:Type u#4) : Type u#4 = address ^-> hogs_val_ x
 
 let fmap #a #b (f:a -> b) 
 : (invariants a ^-> invariants b)
 = F.on_dom (invariants a) fun x ->
     F.on_dom address fun a ->
-      map_istore_val f (x a)
+      map_hogs_val f (x a)
 
 let f_ext #t #s (f g: t ^-> s) (h: (x:t -> squash (f x == g x))) : squash (f == g) =
   introduce forall x. f x == g x with h x;
@@ -73,9 +73,9 @@ let functor_heap : functor u#3 invariants = {
   other = rest;
 }
 
-let istore : Type u#4 = knot_t functor_heap
+let hogs : Type u#4 = knot_t functor_heap
 
-let preworld = istore & rest
+let preworld = hogs & rest
 let world_pred : Type u#4 = preworld ^-> prop
 
 let approx n : (world_pred ^-> world_pred) = approx n
@@ -83,38 +83,38 @@ let approx n : (world_pred ^-> world_pred) = approx n
 let timeless_heap_le (a b: timeless_heap_sig.mem) : prop =
   exists c. timeless_heap_sig.sep.disjoint a c /\ b == timeless_heap_sig.sep.join a c
 
-let istore_val = istore_val_ world_pred
+let hogs_val = hogs_val_ world_pred
 
-let read_istore (is: istore) a : istore_val = unpack is a
-let read (w: preworld) a = read_istore (fst w) a
+let read_hogs (is: hogs) a : hogs_val = unpack is a
+let read (w: preworld) a = read_hogs (fst w) a
 
-let level_istore (is: istore) : GTot nat = level is
-let level_ (w: preworld) : GTot nat = level_istore (fst w)
+let level_hogs (is: hogs) : GTot nat = level is
+let level_ (w: preworld) : GTot nat = level_hogs (fst w)
 
 let approx_def n (p: world_pred) w :
     Lemma (approx n p w == (if level_ w >= n then False else p w))
       [SMTPat (approx n p w)] =
   assert_norm (approx n p w == (if level_ w >= n then False else p w))
 
-let istore_le (x y: istore) : prop =
-  level_istore x == level_istore y /\
-  forall a. istore_val_le (read_istore x a) (read_istore y a)
+let hogs_le (x y: hogs) : prop =
+  level_hogs x == level_hogs y /\
+  forall a. hogs_val_le (read_hogs x a) (read_hogs y a)
 
 let world_le (a b: preworld) : prop =
   let ai, ar = a in
   let bi, br = b in
-  istore_le ai bi /\
+  hogs_le ai bi /\
   timeless_heap_le ar.timeless_heap br.timeless_heap /\
   ar.saved_credits <= br.saved_credits
 
 let world_pred_affine (p: world_pred) : prop =
   forall a b. world_le a b /\ p a ==> p b
 
-let age_istore_to (is: istore) (n: erased nat) : istore =
+let age_hogs_to (is: hogs) (n: erased nat) : hogs =
   pack n (unpack is)
 
 let age_to_ (w: preworld) (n: erased nat) : preworld =
-  (age_istore_to (fst w) n, snd w)
+  (age_hogs_to (fst w) n, snd w)
 
 let hereditary (p: world_pred) : prop =
   forall (w: preworld) (n: erased nat).
@@ -123,40 +123,40 @@ let hereditary (p: world_pred) : prop =
 
 let slprop_ok (p: world_pred) = hereditary p /\ world_pred_affine p
 
-let fresh_addr (is: istore) (a: address) =
-  forall (b: address). b >= a ==> None? (read_istore is b)
+let fresh_addr (is: hogs) (a: address) =
+  forall (b: address). b >= a ==> None? (read_hogs is b)
 
-let istore_bounded (is: istore) =
+let hogs_bounded (is: hogs) =
   exists a. fresh_addr is a
 
-let istore_val_ok (v: istore_val) =
+let hogs_val_ok (v: hogs_val) =
   match v with
   | None -> True
   | Pred p -> slprop_ok p
   | Inv p -> slprop_ok p
 
-let istore_ok (is: istore) : prop =
-  istore_bounded is /\
-  forall a. istore_val_ok (read_istore is a)
+let hogs_ok (is: hogs) : prop =
+  hogs_bounded is /\
+  forall a. hogs_val_ok (read_hogs is a)
 
 let world_ok (w: preworld) : prop =
-  istore_ok (fst w)
+  hogs_ok (fst w)
 
 let slprop = p:world_pred { slprop_ok p }
 
 let world = w:preworld { world_ok w }
 
-let read_age_istore_to (is: istore) (n: erased nat) a : Lemma (read_istore (age_istore_to is n) a ==
-    (map_istore_val (approx n) (read_istore is a)))
-    [SMTPat (read_istore (age_istore_to is n) a)] =
+let read_age_hogs_to (is: hogs) (n: erased nat) a : Lemma (read_hogs (age_hogs_to is n) a ==
+    (map_hogs_val (approx n) (read_hogs is a)))
+    [SMTPat (read_hogs (age_hogs_to is n) a)] =
   unpack_pack n (unpack is)
 
 let read_age_to_ (w: preworld) (n: erased nat) a :
-    Lemma (read (age_to_ w n) a == map_istore_val (approx n) (read w a)) =
+    Lemma (read (age_to_ w n) a == map_hogs_val (approx n) (read w a)) =
   ()
 
-let level_age_istore_to_ is (n: erased nat) :
-    Lemma (level_istore (age_istore_to is n) == reveal n) [SMTPat (level_istore (age_istore_to is n))] =
+let level_age_hogs_to_ is (n: erased nat) :
+    Lemma (level_hogs (age_hogs_to is n) == reveal n) [SMTPat (level_hogs (age_hogs_to is n))] =
   unpack_pack n (unpack is)
 
 let level_age_to_ w (n: erased nat) : Lemma (level_ (age_to_ w n) == reveal n) =
@@ -165,15 +165,15 @@ let level_age_to_ w (n: erased nat) : Lemma (level_ (age_to_ w n) == reveal n) =
 let age_to (w: world) (n: erased nat) : world =
   age_to_ w n
 
-let istore_ext (i1: istore) (i2: istore { level_istore i1 == level_istore i2 })
-    (h: (a:address -> squash (read_istore i1 a == read_istore i2 a))) : squash (i1 == i2) =
+let hogs_ext (i1: hogs) (i2: hogs { level_hogs i1 == level_hogs i2 })
+    (h: (a:address -> squash (read_hogs i1 a == read_hogs i2 a))) : squash (i1 == i2) =
   f_ext (unpack i1) (unpack i2) (fun a -> h a);
   pack_unpack i1;
   pack_unpack i2
 
 let world_ext (w1: preworld) (w2: preworld { level_ w1 == level_ w2 /\ snd w1 == snd w2 })
     (h: (a: address -> squash (read w1 a == read w2 a))) : squash (w1 == w2) =
-  istore_ext (fst w1) (fst w2) h
+  hogs_ext (fst w1) (fst w2) h
 
 let world_pred_ext (f g: world_pred) (h: (w:preworld -> squash (f w <==> g w))) : squash (f == g) =
   f_ext f g fun w ->
@@ -193,32 +193,32 @@ let age_to_rest (w: world) (n: erased nat) : Lemma ((age_to w n)._2 == w._2) = (
 let level (w: world) : GTot nat = level_ w
 
 irreducible [@@"opaque_to_smt"]
-let reveal_istore (is: erased istore) : is':istore { is' == reveal is } =
+let reveal_hogs (is: erased hogs) : is':hogs { is' == reveal is } =
   pack_unpack is;
   pack (IT.level is) (unpack is)
 
-let approx_read_istore (is: istore) a :
-    Lemma (map_istore_val (approx (level_istore is)) (read_istore is a) == read_istore is a)
-    [SMTPat (read_istore is a)] =
-  pack_unpack is; unpack_pack (level_istore is) (unpack is)
+let approx_read_hogs (is: hogs) a :
+    Lemma (map_hogs_val (approx (level_hogs is)) (read_hogs is a) == read_hogs is a)
+    [SMTPat (read_hogs is a)] =
+  pack_unpack is; unpack_pack (level_hogs is) (unpack is)
 
-let age1_istore (is: istore) : is':istore { level_istore is == 0 ==> is' == is } =
-  istore_ext (age_istore_to is (level_istore is)) is (fun _ -> ());
-  age_istore_to is (if level_istore is > 0 then level_istore is - 1 else 0)
+let age1_hogs (is: hogs) : is':hogs { level_hogs is == 0 ==> is' == is } =
+  hogs_ext (age_hogs_to is (level_hogs is)) is (fun _ -> ());
+  age_hogs_to is (if level_hogs is > 0 then level_hogs is - 1 else 0)
 
-let istore_ok_age1 (is: istore) :
-    Lemma (requires istore_ok is) (ensures istore_ok (age1_istore is)) [SMTPat (istore_ok (age1_istore is))] =
+let hogs_ok_age1 (is: hogs) :
+    Lemma (requires hogs_ok is) (ensures hogs_ok (age1_hogs is)) [SMTPat (hogs_ok (age1_hogs is))] =
   ()
 
 let age1_ (w: preworld) : w':preworld { if level_ w > 0 then w' == age_to_ w (level_ w - 1) else w' == w } =
-  (age1_istore (fst w), snd w)
+  (age1_hogs (fst w), snd w)
 
 let age1 (w: world) : world = age1_ w
 
 let credits (w: world) : GTot nat =
   w._2.saved_credits
 
-let okay_istore = is:istore { istore_ok is }
+let okay_hogs = is:hogs { hogs_ok is }
 
 let eq_at (n:nat) (t0 t1:world_pred) =
   approx n t0 == approx n t1
@@ -232,43 +232,43 @@ let eq_at_mono (p q: world_pred) m n :
 let interp p w = p w
 
 unfold
-let istore_val_compat (x y: istore_val) =
+let hogs_val_compat (x y: hogs_val) =
   match x, y with
   | None, _ | _, None -> True
   | Pred p0, Pred p1 -> p0 == p1
   | Inv p0, Inv p1 -> p0 == p1
   | Inv _, Pred _ | Pred _, Inv _ -> False
 
-let disjoint_istore (is0 is1:istore) =
-  level_istore is0 == level_istore is1 /\
-  (forall a. istore_val_compat (read_istore is0 a) (read_istore is1 a))
+let disjoint_hogs (is0 is1:hogs) =
+  level_hogs is0 == level_hogs is1 /\
+  (forall a. hogs_val_compat (read_hogs is0 a) (read_hogs is1 a))
 
-let disjoint_istore_read is0 is1 a :
-    Lemma (requires disjoint_istore is0 is1)
-      (ensures istore_val_compat (read_istore is0 a) (read_istore is1 a))
+let disjoint_hogs_read is0 is1 a :
+    Lemma (requires disjoint_hogs is0 is1)
+      (ensures hogs_val_compat (read_hogs is0 a) (read_hogs is1 a))
       [SMTPatOr [
-        [SMTPat (disjoint_istore is0 is1); SMTPat (read_istore is0 a)];
-        [SMTPat (disjoint_istore is0 is1); SMTPat (read_istore is1 a)];
+        [SMTPat (disjoint_hogs is0 is1); SMTPat (read_hogs is0 a)];
+        [SMTPat (disjoint_hogs is0 is1); SMTPat (read_hogs is1 a)];
       ]] =
   ()
 
-let mk_istore n (is: address -> istore_val) : istore =
+let mk_hogs n (is: address -> hogs_val) : hogs =
   pack n (F.on_dom address is)
 
-let level_mk_istore (n: erased nat) is :
-    Lemma (level_istore (mk_istore n is) == reveal n) [SMTPat (level_istore (mk_istore n is))] =
+let level_mk_hogs (n: erased nat) is :
+    Lemma (level_hogs (mk_hogs n is) == reveal n) [SMTPat (level_hogs (mk_hogs n is))] =
   unpack_pack #_ #functor_heap n (F.on_dom address is)
 
-let read_mk_istore (n: erased nat) is a :
-    Lemma (read_istore (mk_istore n is) a == map_istore_val (approx n) (is a))
-      [SMTPat (read_istore (mk_istore n is) a)] =
+let read_mk_hogs (n: erased nat) is a :
+    Lemma (read_hogs (mk_hogs n is) a == map_hogs_val (approx n) (is a))
+      [SMTPat (read_hogs (mk_hogs n is) a)] =
   let is' = F.on_dom address is in
   unpack_pack #_ #functor_heap n is';
-  assert_norm (fmap (approx n) is' a == map_istore_val (approx n) (is' a))
+  assert_norm (fmap (approx n) is' a == map_hogs_val (approx n) (is' a))
 
-let empty_istore n : istore = mk_istore n fun _ -> None
+let empty_hogs n : hogs = mk_hogs n fun _ -> None
 let empty_rest : rest = { timeless_heap = timeless_heap_sig.sep.empty; saved_credits = 0 }
-let empty n : world = (empty_istore n, empty_rest)
+let empty n : world = (empty_hogs n, empty_rest)
 
 let age_to_empty (m n: erased nat) : Lemma (age_to (empty n) m == empty m) [SMTPat (age_to (empty n) m)] =
   world_ext (age_to (empty n) m) (empty m) fun a -> read_age_to_ (empty n) m a
@@ -278,52 +278,52 @@ let emp : slprop =
 
 let pure p : slprop = F.on_dom _ fun w -> p
 
-let join_istore (is0:istore) (is1:istore { disjoint_istore is0 is1 }) : istore =
-  mk_istore (level_istore is0) fun a ->
-    match read_istore is0 a, read_istore is1 a with
+let join_hogs (is0:hogs) (is1:hogs { disjoint_hogs is0 is1 }) : hogs =
+  mk_hogs (level_hogs is0) fun a ->
+    match read_hogs is0 a, read_hogs is1 a with
     | None, None -> None
     | Pred p, _ | _, Pred p -> Pred p
     | Inv p, _ | _, Inv p -> Inv p
 
-let read_join_istore (is0:istore) (is1:istore { disjoint_istore is0 is1 }) a :
-  Lemma (read_istore (join_istore is0 is1) a ==
-    (match read_istore is0 a, read_istore is1 a with
+let read_join_hogs (is0:hogs) (is1:hogs { disjoint_hogs is0 is1 }) a :
+  Lemma (read_hogs (join_hogs is0 is1) a ==
+    (match read_hogs is0 a, read_hogs is1 a with
     | None, None -> None
-    | Pred p, _ | _, Pred p -> Pred (approx (level_istore is0) p)
-    | Inv p, _ | _, Inv p -> Inv (approx (level_istore is0) p))) =
+    | Pred p, _ | _, Pred p -> Pred (approx (level_hogs is0) p)
+    | Inv p, _ | _, Inv p -> Inv (approx (level_hogs is0) p))) =
   ()
 
-let join_istore_commutative (is0:istore) (is1:istore { disjoint_istore is0 is1 }) :
-    Lemma (join_istore is0 is1 == join_istore is1 is0) =
-  istore_ext (join_istore is0 is1) (join_istore is1 is0) fun a -> ()
+let join_hogs_commutative (is0:hogs) (is1:hogs { disjoint_hogs is0 is1 }) :
+    Lemma (join_hogs is0 is1 == join_hogs is1 is0) =
+  hogs_ext (join_hogs is0 is1) (join_hogs is1 is0) fun a -> ()
 
-let join_istore_refl (is: istore) : Lemma (disjoint_istore is is /\ join_istore is is == is) =
-  istore_ext (join_istore is is) is fun a -> ()
+let join_hogs_refl (is: hogs) : Lemma (disjoint_hogs is is /\ join_hogs is is == is) =
+  hogs_ext (join_hogs is is) is fun a -> ()
 
-let join_istore_associative
-    (is0:istore)
-    (is1:istore)
-    (is2:istore { 
-      disjoint_istore is1 is2 /\
-      disjoint_istore is0 (join_istore is1 is2)
+let join_hogs_associative
+    (is0:hogs)
+    (is1:hogs)
+    (is2:hogs { 
+      disjoint_hogs is1 is2 /\
+      disjoint_hogs is0 (join_hogs is1 is2)
     })
 : Lemma (
-    disjoint_istore is0 is1 /\
-    disjoint_istore (join_istore is0 is1) is2 /\
-    join_istore is0 (join_istore is1 is2) ==
-    join_istore (join_istore is0 is1) is2
+    disjoint_hogs is0 is1 /\
+    disjoint_hogs (join_hogs is0 is1) is2 /\
+    join_hogs is0 (join_hogs is1 is2) ==
+    join_hogs (join_hogs is0 is1) is2
   )
 =
-  istore_ext (join_istore is0 (join_istore is1 is2)) (join_istore (join_istore is0 is1) is2) fun a -> ()
+  hogs_ext (join_hogs is0 (join_hogs is1 is2)) (join_hogs (join_hogs is0 is1) is2) fun a -> ()
 
-let istore_le_iff (is1 is2: istore) :
-    Lemma (istore_le is1 is2 <==> exists is3. join_istore is1 is3 == is2) =
-  introduce istore_le is1 is2 ==> exists is3. join_istore is1 is3 == is2 with _.
-    istore_ext (join_istore is1 is2) is2 fun _ -> ()
+let hogs_le_iff (is1 is2: hogs) :
+    Lemma (hogs_le is1 is2 <==> exists is3. join_hogs is1 is3 == is2) =
+  introduce hogs_le is1 is2 ==> exists is3. join_hogs is1 is3 == is2 with _.
+    hogs_ext (join_hogs is1 is2) is2 fun _ -> ()
 
 let disjoint_worlds (w0 w1:preworld)
 : prop 
-= disjoint_istore w0._1 w1._1 /\
+= disjoint_hogs w0._1 w1._1 /\
   timeless_heap_sig.sep.disjoint w0._2.timeless_heap w1._2.timeless_heap
 
 let disjoint_world_sym (w0 w1:preworld)
@@ -333,7 +333,7 @@ let disjoint_world_sym (w0 w1:preworld)
 
 let join_worlds (w0:preworld) (w1:preworld { disjoint_worlds w0 w1 })
 : preworld
-= (join_istore w0._1 w1._1, ({
+= (join_hogs w0._1 w1._1, ({
     timeless_heap = timeless_heap_sig.sep.join w0._2.timeless_heap w1._2.timeless_heap;
     saved_credits = w0._2.saved_credits + w1._2.saved_credits } <: rest))
 
@@ -341,13 +341,13 @@ open FStar.IndefiniteDescription { indefinite_description_ghost, strong_excluded
 
 let world_le_iff (w1 w2: preworld) :
     Lemma (world_le w1 w2 <==> exists w3. join_worlds w1 w3 == w2) =
-  istore_le_iff (fst w1) (fst w2);
+  hogs_le_iff (fst w1) (fst w2);
   introduce world_le w1 w2 ==> exists w3. join_worlds w1 w3 == w2 with _. (
     assert timeless_heap_le (snd w1).timeless_heap (snd w2).timeless_heap;
     let ph3 = indefinite_description_ghost _ fun ph3 ->
       (snd w2).timeless_heap == timeless_heap_sig.sep.join (snd w1).timeless_heap ph3 in
     let is3 = indefinite_description_ghost _ fun is3 ->
-      fst w2 == join_istore (fst w1) is3 in
+      fst w2 == join_hogs (fst w1) is3 in
     let sc3: nat = (snd w2).saved_credits - (snd w1).saved_credits in
     let w3: preworld = (is3, ({ timeless_heap = ph3; saved_credits = sc3 } <: rest)) in
     assert join_worlds w1 w3 == w2
@@ -356,7 +356,7 @@ let world_le_iff (w1 w2: preworld) :
 let join_worlds_commutative (w0:preworld) (w1:preworld { disjoint_worlds w0 w1 })
 : Lemma (disjoint_worlds w1 w0 /\ join_worlds w0 w1 == join_worlds w1 w0)
 = disjoint_world_sym w0 w1;
-  join_istore_commutative w0._1 w1._1;
+  join_hogs_commutative w0._1 w1._1;
   timeless_heap_sig.sep.join_commutative w0._2.timeless_heap w1._2.timeless_heap
 
 let join_worlds_associative
@@ -369,7 +369,7 @@ let join_worlds_associative
     join_worlds w0 (join_worlds w1 w2) ==
     join_worlds (join_worlds w0 w1) w2
   )
-= join_istore_associative w0._1 w1._1 w2._1;
+= join_hogs_associative w0._1 w1._1 w2._1;
   timeless_heap_sig.sep.join_associative w0._2.timeless_heap w1._2.timeless_heap w2._2.timeless_heap
 
 let age_to_disjoint_worlds (w1 w2: preworld) n :
@@ -377,12 +377,12 @@ let age_to_disjoint_worlds (w1 w2: preworld) n :
       (ensures disjoint_worlds (age_to_ w1 n) (age_to_ w2 n)) =
   ()
 
-let age_to_istore_join (i1 i2: istore) n :
-    Lemma (requires disjoint_istore i1 i2)
-      (ensures disjoint_istore (age_istore_to i1 n) (age_istore_to i2 n) /\
-        age_istore_to (join_istore i1 i2) n == join_istore (age_istore_to i1 n) (age_istore_to i2 n))
-    [SMTPat (age_istore_to (join_istore i1 i2) n)] =
-  istore_ext (age_istore_to (join_istore i1 i2) n) (join_istore (age_istore_to i1 n) (age_istore_to i2 n)) fun a -> ()
+let age_to_hogs_join (i1 i2: hogs) n :
+    Lemma (requires disjoint_hogs i1 i2)
+      (ensures disjoint_hogs (age_hogs_to i1 n) (age_hogs_to i2 n) /\
+        age_hogs_to (join_hogs i1 i2) n == join_hogs (age_hogs_to i1 n) (age_hogs_to i2 n))
+    [SMTPat (age_hogs_to (join_hogs i1 i2) n)] =
+  hogs_ext (age_hogs_to (join_hogs i1 i2) n) (join_hogs (age_hogs_to i1 n) (age_hogs_to i2 n)) fun a -> ()
 
 let age_to_join (w1 w2: preworld) n :
     Lemma (requires disjoint_worlds w1 w2)
@@ -479,10 +479,10 @@ let star_assoc (x y z:slprop)
 : Lemma (star x (star y z) == star (star x y) z)
 = star__assoc x y z
 
-let disjoint_istore_empty is : squash (disjoint_istore (empty_istore (level_istore is)) is) = ()
+let disjoint_hogs_empty is : squash (disjoint_hogs (empty_hogs (level_hogs is)) is) = ()
 
-let join_istore_empty is : squash (join_istore (empty_istore (level_istore is)) is == is) =
-  istore_ext (join_istore (empty_istore (level_istore is)) is) is fun a -> ()
+let join_hogs_empty is : squash (join_hogs (empty_hogs (level_hogs is)) is == is) =
+  hogs_ext (join_hogs (empty_hogs (level_hogs is)) is) is fun a -> ()
 
 let disjoint_empty w : squash (disjoint_worlds w (empty (level_ w)) /\ disjoint_worlds (empty (level_ w)) w) =
   timeless_heap_sig.sep.join_empty w._2.timeless_heap;
@@ -492,7 +492,7 @@ let join_empty w : squash (disjoint_worlds (empty (level_ w)) w /\ join_worlds (
   disjoint_empty w;
   timeless_heap_sig.sep.join_empty w._2.timeless_heap;
   timeless_heap_sig.sep.join_commutative w._2.timeless_heap timeless_heap_sig.sep.empty;
-  join_istore_empty w._1;
+  join_hogs_empty w._1;
   world_ext (join_worlds (empty (level_ w)) w) w fun a -> ()
 
 let star_emp (x: slprop) : squash (star x emp == x) =
@@ -547,7 +547,7 @@ let lift_star_eq p q =
       let w0: preworld = (fst w, ({ snd w with timeless_heap = m0 } <: rest)) in
       let w1: preworld = (fst w, ({ timeless_heap = m1; saved_credits = 0 } <: rest)) in
       assert disjoint_worlds w0 w1;
-      join_istore_refl (fst w);
+      join_hogs_refl (fst w);
       assert join_worlds w0 w1 == w;
       assert lift p w0;
       assert lift q w1;
@@ -677,31 +677,31 @@ let equiv_timeless (a b: slprop) :
       timeless_ext a b fun w' ->
         eq_at_elim 1 a b w'
 
-let rejuvenate1_istore (is: istore) (is': istore { istore_le is' (age1_istore is) }) :
-    is'':istore { age1_istore is'' == is' /\ istore_le is'' is } =
-  let is'' = mk_istore (level_istore is) fun a -> if None? (read_istore is' a) then None else read_istore is a in
-  istore_ext (age1_istore is'') is' (fun a -> ());
+let rejuvenate1_hogs (is: hogs) (is': hogs { hogs_le is' (age1_hogs is) }) :
+    is'':hogs { age1_hogs is'' == is' /\ hogs_le is'' is } =
+  let is'' = mk_hogs (level_hogs is) fun a -> if None? (read_hogs is' a) then None else read_hogs is a in
+  hogs_ext (age1_hogs is'') is' (fun a -> ());
   is''
 
-let rejuvenate1_istore_sep (is is1': istore) (is2': istore { disjoint_istore is1' is2' /\ age1_istore is == join_istore is1' is2' }) :
-    is'':(istore&istore) { age1_istore is''._1 == is1' /\ age1_istore is''._2 == is2'
-      /\ disjoint_istore is''._1 is''._2 /\ is == join_istore is''._1 is''._2 } =
-  let is1'' = rejuvenate1_istore is is1' in
-  join_istore_commutative is1' is2';
-  let is2'' = rejuvenate1_istore is is2' in
-  assert disjoint_istore is1'' is2'';
-  istore_ext is (join_istore is1'' is2'') (fun a ->
-    assert ~(None? (read_istore is1'' a)) ==> read_istore is a == read_istore is1'' a);
+let rejuvenate1_hogs_sep (is is1': hogs) (is2': hogs { disjoint_hogs is1' is2' /\ age1_hogs is == join_hogs is1' is2' }) :
+    is'':(hogs&hogs) { age1_hogs is''._1 == is1' /\ age1_hogs is''._2 == is2'
+      /\ disjoint_hogs is''._1 is''._2 /\ is == join_hogs is''._1 is''._2 } =
+  let is1'' = rejuvenate1_hogs is is1' in
+  join_hogs_commutative is1' is2';
+  let is2'' = rejuvenate1_hogs is is2' in
+  assert disjoint_hogs is1'' is2'';
+  hogs_ext is (join_hogs is1'' is2'') (fun a ->
+    assert ~(None? (read_hogs is1'' a)) ==> read_hogs is a == read_hogs is1'' a);
   (is1'', is2'')
 
 let rejuvenate1 (w: preworld) (w': preworld { world_le w' (age1_ w) }) :
     w'':preworld { age1_ w'' == w' /\ world_le w'' w /\ snd w'' == snd w' } =
-  (rejuvenate1_istore (fst w) (fst w'), snd w')
+  (rejuvenate1_hogs (fst w) (fst w'), snd w')
 
 let rejuvenate1_sep (w w1': preworld) (w2': preworld { disjoint_worlds w1' w2' /\ age1_ w == join_worlds w1' w2' }) :
     w'':(preworld&preworld) { age1_ w''._1 == w1' /\ age1_ w''._2 == w2'
       /\ disjoint_worlds w''._1 w''._2 /\ w == join_worlds w''._1 w''._2 } =
-  let (is1'', is2'') = rejuvenate1_istore_sep (fst w) (fst w1') (fst w2') in
+  let (is1'', is2'') = rejuvenate1_hogs_sep (fst w) (fst w1') (fst w2') in
   ((is1'', snd w1'), (is2'', snd w2'))
 
 let later_star (p q: slprop) : squash (later (star p q) == star (later p) (later q)) =
@@ -718,10 +718,10 @@ let later_exists #t (f:t->slprop) : squash (later (exists* x. f x) == (exists* x
 
 let iref = address
 
-let inv_prop (i:iref) (p:slprop) (is:istore) : prop =
+let inv_prop (i:iref) (p:slprop) (is:hogs) : prop =
   exists p'.
-    read_istore is i == Inv p' /\
-    eq_at (level_istore is) p p'
+    read_hogs is i == Inv p' /\
+    eq_at (level_hogs is) p p'
 
 let inv (i:iref) (p:slprop) : slprop =
   F.on_dom preworld #(fun _ -> prop) fun w -> inv_prop i p (fst w)
@@ -733,242 +733,242 @@ let inames_dec_eq : GS.decide_eq address = fun x y -> reveal x = reveal y
 let single (i:iref) : inames = GS.singleton inames_dec_eq i
 let add_inv (e:inames) (i:iref) : inames = GS.union (single i) e
 
-let iname_ok (i: iref) (is: istore) =
-  Inv? (read_istore is i)
+let iname_ok (i: iref) (is: hogs) =
+  Inv? (read_hogs is i)
 
-let read_inv (i: iref) (is: okay_istore { iname_ok i is }) : slprop =
-  let Inv p = read_istore is i in p
+let read_inv (i: iref) (is: okay_hogs { iname_ok i is }) : slprop =
+  let Inv p = read_hogs is i in p
 
 let read_inv_equiv i (w: world { level_ w > 0 }) (p: slprop) :
     Lemma (requires inv i p w)
       (ensures eq_at (level_ w) (read_inv i (fst w)) p) =
   ()
 
-let inames_ok (e: inames) (is: istore) : prop =
+let inames_ok (e: inames) (is: hogs) : prop =
   forall a. GS.mem a e ==> iname_ok a is
 
-let istore_dom (is: istore) : inames =
-  GS.comprehend fun a -> Inv? (read_istore is a)
+let hogs_dom (is: hogs) : inames =
+  GS.comprehend fun a -> Inv? (read_hogs is a)
 
-let rec istore_invariant_ (ex: inames) (is: okay_istore) (f: address) : slprop =
+let rec hogs_invariant_ (ex: inames) (is: okay_hogs) (f: address) : slprop =
   if reveal f = 0 then
     emp
   else
     let f': address = f - 1 in
     if GS.mem f' ex then
-      istore_invariant_ ex is f'
+      hogs_invariant_ ex is f'
     else
-      match read_istore is f' with
-      | Inv p -> later p `star` istore_invariant_ ex is f'
-      | _ -> istore_invariant_ ex is f'
+      match read_hogs is f' with
+      | Inv p -> later p `star` hogs_invariant_ ex is f'
+      | _ -> hogs_invariant_ ex is f'
 
-let rec istore_invariant__congr (ex: inames) (m: okay_istore) (f1 f2: (f:address { fresh_addr m f })) :
-    Lemma (ensures istore_invariant_ ex m f1 == istore_invariant_ ex m f2) (decreases f1+f2+f2) =
+let rec hogs_invariant__congr (ex: inames) (m: okay_hogs) (f1 f2: (f:address { fresh_addr m f })) :
+    Lemma (ensures hogs_invariant_ ex m f1 == hogs_invariant_ ex m f2) (decreases f1+f2+f2) =
   if f1 < f2 then
-    istore_invariant__congr ex m f2 f1
+    hogs_invariant__congr ex m f2 f1
   else if f1 > f2 then
-    istore_invariant__congr ex m (f1 - 1) f2
+    hogs_invariant__congr ex m (f1 - 1) f2
   else
     ()
 
-[@@"opaque_to_smt"] irreducible let some_fresh_addr (is: okay_istore) : a:address { fresh_addr is a } =
+[@@"opaque_to_smt"] irreducible let some_fresh_addr (is: okay_hogs) : a:address { fresh_addr is a } =
   indefinite_description_ghost address fun a -> fresh_addr is a
 
-let istore_invariant (ex: inames) (is: okay_istore) : slprop =
-  istore_invariant_ ex is (some_fresh_addr is)
+let hogs_invariant (ex: inames) (is: okay_hogs) : slprop =
+  hogs_invariant_ ex is (some_fresh_addr is)
 
-let rec istore_invariant__equiv (ex: inames) (m: okay_istore) (i:iref { iname_ok i m /\ ~(GS.mem i ex) }) (f: address) :
-    Lemma (istore_invariant_ ex m f ==
+let rec hogs_invariant__equiv (ex: inames) (m: okay_hogs) (i:iref { iname_ok i m /\ ~(GS.mem i ex) }) (f: address) :
+    Lemma (hogs_invariant_ ex m f ==
       (if i < f then
-        istore_invariant_ (add_inv ex i) m f `star` later (read_inv i m)
+        hogs_invariant_ (add_inv ex i) m f `star` later (read_inv i m)
       else
-        istore_invariant_ (add_inv ex i) m f)) =
+        hogs_invariant_ (add_inv ex i) m f)) =
   if reveal f = 0 then
     ()
   else
     let f': address = f - 1 in
-    istore_invariant__equiv ex m i f';
+    hogs_invariant__equiv ex m i f';
     if GS.mem f' ex then
       ()
     else
-      match read_istore m f' with
+      match read_hogs m f' with
       | Inv p -> sep_laws ()
       | _ -> ()
 
-let istore_invariant_equiv (ex: inames) (m: okay_istore) (i:iref { iname_ok i m /\ ~(GS.mem i ex) }) :
-    Lemma (istore_invariant ex m ==
-      istore_invariant (add_inv ex i) m `star` later (read_inv i m)) =
-  istore_invariant__equiv ex m i (some_fresh_addr m)
+let hogs_invariant_equiv (ex: inames) (m: okay_hogs) (i:iref { iname_ok i m /\ ~(GS.mem i ex) }) :
+    Lemma (hogs_invariant ex m ==
+      hogs_invariant (add_inv ex i) m `star` later (read_inv i m)) =
+  hogs_invariant__equiv ex m i (some_fresh_addr m)
 
-let rec istore_invariant__age (e:inames) (is: okay_istore { level_istore is > 0 }) (f: address) :
-    Lemma (forall w. 1 < level_ w /\ level_ w <= level_istore is /\ istore_invariant_ e is f w ==>
-        istore_invariant_ e (age1_istore is) f (age1_ w)) =
+let rec hogs_invariant__age (e:inames) (is: okay_hogs { level_hogs is > 0 }) (f: address) :
+    Lemma (forall w. 1 < level_ w /\ level_ w <= level_hogs is /\ hogs_invariant_ e is f w ==>
+        hogs_invariant_ e (age1_hogs is) f (age1_ w)) =
   if reveal f = 0 then
     ()
   else
     let f': address = f - 1 in
-    istore_invariant__age e is f';
+    hogs_invariant__age e is f';
     if GS.mem f' e then
       ()
     else
-      match read_istore is f' with
+      match read_hogs is f' with
       | Inv p ->
-        let Inv p' = read_istore (age1_istore is) f' in
-        assert eq_at (level_istore is - 1) p p';
-        introduce forall (w:preworld { 1 < level_ w /\ level_ w <= level_istore is /\ istore_invariant_ e is f w }).
-            istore_invariant_ e (age1_istore is) f (age1_ w) with (
-          let (w1, w2) = star_elim (later p) (istore_invariant_ e is f') w in
-          assert istore_invariant_ e (age1_istore is) f' (age1_ w2);
+        let Inv p' = read_hogs (age1_hogs is) f' in
+        assert eq_at (level_hogs is - 1) p p';
+        introduce forall (w:preworld { 1 < level_ w /\ level_ w <= level_hogs is /\ hogs_invariant_ e is f w }).
+            hogs_invariant_ e (age1_hogs is) f (age1_ w) with (
+          let (w1, w2) = star_elim (later p) (hogs_invariant_ e is f') w in
+          assert hogs_invariant_ e (age1_hogs is) f' (age1_ w2);
           assert p (age1_ w1);
-          eq_at_elim (level_istore is - 1) p p' (age1_ (age1_ w1));
-          star_intro (later (later p')) (later (istore_invariant_ e (age1_istore is) f')) w w1 w2;
-          later_star (later p') (istore_invariant_ e (age1_istore is) f');
-          assert (later p' `star` istore_invariant_ e (age1_istore is) f') (age1_ w)
+          eq_at_elim (level_hogs is - 1) p p' (age1_ (age1_ w1));
+          star_intro (later (later p')) (later (hogs_invariant_ e (age1_hogs is) f')) w w1 w2;
+          later_star (later p') (hogs_invariant_ e (age1_hogs is) f');
+          assert (later p' `star` hogs_invariant_ e (age1_hogs is) f') (age1_ w)
         )
       | _ ->
         ()
 
-let istore_invariant_age (e:inames) (is: okay_istore { level_istore is > 0 })
-    (w: preworld { 1 < level_ w /\ level_ w <= level_istore is }) :
-    Lemma (istore_invariant e is w ==> istore_invariant e (age1_istore is) (age1_ w)) =
-  introduce istore_invariant e is w ==> istore_invariant e (age1_istore is) (age1_ w) with _. (
-    istore_invariant__age e is (some_fresh_addr is);
-    istore_invariant__congr e (age1_istore is) (some_fresh_addr is) (some_fresh_addr (age1_istore is))
+let hogs_invariant_age (e:inames) (is: okay_hogs { level_hogs is > 0 })
+    (w: preworld { 1 < level_ w /\ level_ w <= level_hogs is }) :
+    Lemma (hogs_invariant e is w ==> hogs_invariant e (age1_hogs is) (age1_ w)) =
+  introduce hogs_invariant e is w ==> hogs_invariant e (age1_hogs is) (age1_ w) with _. (
+    hogs_invariant__age e is (some_fresh_addr is);
+    hogs_invariant__congr e (age1_hogs is) (some_fresh_addr is) (some_fresh_addr (age1_hogs is))
   )
 
 let gs_disjoint_elim #t (a: GS.set t) (b: GS.set t { GS.disjoint a b }) (x: t { GS.mem x a }) :
     Lemma (~(GS.mem x b)) =
   ()
 
-let rec istore_invariant__disjoint (e1 e2:inames) (m1 m2:okay_istore) (f: iref) :
+let rec hogs_invariant__disjoint (e1 e2:inames) (m1 m2:okay_hogs) (f: iref) :
     Lemma (requires
-      disjoint_istore m1 m2 /\
-      GS.disjoint (istore_dom m1) (istore_dom m2) /\
-      GS.disjoint e1 (istore_dom m2) /\ GS.disjoint e2 (istore_dom m1))
+      disjoint_hogs m1 m2 /\
+      GS.disjoint (hogs_dom m1) (hogs_dom m2) /\
+      GS.disjoint e1 (hogs_dom m2) /\ GS.disjoint e2 (hogs_dom m1))
     (ensures 
-      istore_invariant_ (GS.union e1 e2) (join_istore m1 m2) f ==
-        istore_invariant_ e1 m1 f `star` istore_invariant_ e2 m2 f) =
+      hogs_invariant_ (GS.union e1 e2) (join_hogs m1 m2) f ==
+        hogs_invariant_ e1 m1 f `star` hogs_invariant_ e2 m2 f) =
   if reveal f = 0 then
     sep_laws ()
   else
     let f': address = f - 1 in
-    istore_invariant__disjoint e1 e2 m1 m2 f';
+    hogs_invariant__disjoint e1 e2 m1 m2 f';
     if GS.mem f' (GS.union e1 e2) then
       ()
     else
-      match read_istore (join_istore m1 m2) f' with
+      match read_hogs (join_hogs m1 m2) f' with
       | Inv p -> 
-        if Inv? (read_istore m1 f') then (
-          gs_disjoint_elim (istore_dom m1) (istore_dom m2) f';
+        if Inv? (read_hogs m1 f') then (
+          gs_disjoint_elim (hogs_dom m1) (hogs_dom m2) f';
           sep_laws ()
-        ) else if Inv? (read_istore m2 f') then (
-          gs_disjoint_elim (istore_dom m2) (istore_dom m1) f';
+        ) else if Inv? (read_hogs m2 f') then (
+          gs_disjoint_elim (hogs_dom m2) (hogs_dom m1) f';
           sep_laws ()
         ) else
           assert False
       | _ -> ()
 
-let istore_invariant_disjoint (e1 e2:inames) (m1 m2:okay_istore) :
+let hogs_invariant_disjoint (e1 e2:inames) (m1 m2:okay_hogs) :
     Lemma (requires
-      disjoint_istore m1 m2 /\
-      GS.disjoint (istore_dom m1) (istore_dom m2) /\
-      GS.disjoint e1 (istore_dom m2) /\ GS.disjoint e2 (istore_dom m1))
+      disjoint_hogs m1 m2 /\
+      GS.disjoint (hogs_dom m1) (hogs_dom m2) /\
+      GS.disjoint e1 (hogs_dom m2) /\ GS.disjoint e2 (hogs_dom m1))
     (ensures 
-      istore_invariant (GS.union e1 e2) (join_istore m1 m2) ==
-        istore_invariant e1 m1 `star` istore_invariant e2 m2) =
-  let m = join_istore m1 m2 in
-  istore_invariant__congr e1 m1 (some_fresh_addr m1) (some_fresh_addr m);
-  istore_invariant__congr e2 m2 (some_fresh_addr m2) (some_fresh_addr m);
-  istore_invariant__disjoint e1 e2 m1 m2 (some_fresh_addr m)
+      hogs_invariant (GS.union e1 e2) (join_hogs m1 m2) ==
+        hogs_invariant e1 m1 `star` hogs_invariant e2 m2) =
+  let m = join_hogs m1 m2 in
+  hogs_invariant__congr e1 m1 (some_fresh_addr m1) (some_fresh_addr m);
+  hogs_invariant__congr e2 m2 (some_fresh_addr m2) (some_fresh_addr m);
+  hogs_invariant__disjoint e1 e2 m1 m2 (some_fresh_addr m)
 
-let rec istore_invariant__mono (ex1: inames) (ex2: inames)
-    (m: okay_istore { forall i. GS.mem i (istore_dom m) /\ GS.mem i ex1 ==> GS.mem i ex2 })
+let rec hogs_invariant__mono (ex1: inames) (ex2: inames)
+    (m: okay_hogs { forall i. GS.mem i (hogs_dom m) /\ GS.mem i ex1 ==> GS.mem i ex2 })
     (f: address) (w: preworld) :
-    squash (istore_invariant_ ex1 m f w ==> istore_invariant_ ex2 m f w) =
+    squash (hogs_invariant_ ex1 m f w ==> hogs_invariant_ ex2 m f w) =
   introduce _ ==> _ with _.
   if reveal f = 0 then
     ()
   else
     let f': address = f - 1 in
     if GS.mem f' ex1 then
-      istore_invariant__mono ex1 ex2 m f' w
+      hogs_invariant__mono ex1 ex2 m f' w
     else
-      match read_istore m f' with
+      match read_hogs m f' with
       | Inv p ->
-        let (w1, w2) = star_elim (later p) (istore_invariant_ ex1 m f') w in
-        istore_invariant__mono ex1 ex2 m f' w2;
+        let (w1, w2) = star_elim (later p) (hogs_invariant_ ex1 m f') w in
+        hogs_invariant__mono ex1 ex2 m f' w2;
         join_worlds_commutative w1 w2;
         assert world_le w2 w
       | _ ->
-        istore_invariant__mono ex1 ex2 m f' w
+        hogs_invariant__mono ex1 ex2 m f' w
 
-let istore_invariant_mono (ex1: inames) (ex2: inames)
-    (m: okay_istore { forall i. GS.mem i (istore_dom m) /\ GS.mem i ex1 ==> GS.mem i ex2 })
+let hogs_invariant_mono (ex1: inames) (ex2: inames)
+    (m: okay_hogs { forall i. GS.mem i (hogs_dom m) /\ GS.mem i ex1 ==> GS.mem i ex2 })
     (w: preworld) :
-    squash (istore_invariant ex1 m w ==> istore_invariant ex2 m w) =
-  istore_invariant__mono ex1 ex2 m (some_fresh_addr m) w
+    squash (hogs_invariant ex1 m w ==> hogs_invariant ex2 m w) =
+  hogs_invariant__mono ex1 ex2 m (some_fresh_addr m) w
 
 let gs_diff #t (a b: GS.set t) : GS.set t =
   GS.comprehend fun i -> GS.mem i a && not (GS.mem i b)
 
-let istore_invariant_disjoint' (e f:inames) (p0 p1:slprop) (m0 m1:world) :
+let hogs_invariant_disjoint' (e f:inames) (p0 p1:slprop) (m0 m1:world) :
     Lemma (requires
       disjoint_worlds m0 m1 /\
-      GS.disjoint (istore_dom (fst m0)) (istore_dom (fst m1)) /\
-      (p0 `star` istore_invariant e (fst m0)) m0 /\
-      (p1 `star` istore_invariant f (fst m1)) m1)
+      GS.disjoint (hogs_dom (fst m0)) (hogs_dom (fst m1)) /\
+      (p0 `star` hogs_invariant e (fst m0)) m0 /\
+      (p1 `star` hogs_invariant f (fst m1)) m1)
     (ensures (
       let m = join_worlds m0 m1 in
-      (p0 `star` p1 `star` istore_invariant (GS.union e f) (fst m)) m)) =
-  let e' = gs_diff e (istore_dom (fst m1)) in
-  let _ : squash ((p0 `star` istore_invariant e' (fst m0)) m0) =
-    let (w1, w2) = star_elim p0 (istore_invariant e (fst m0)) m0 in
-    istore_invariant_mono e e' (fst m0) w2;
-    star_intro p0 (istore_invariant e' (fst m0)) m0 w1 w2 in
-  let f' = gs_diff f (istore_dom (fst m0)) in
-  let _ : squash ((p1 `star` istore_invariant f' (fst m1)) m1) =
-    let (w1, w2) = star_elim p1 (istore_invariant f (fst m1)) m1 in
-    istore_invariant_mono f f' (fst m1) w2;
-    star_intro p1 (istore_invariant f' (fst m1)) m1 w1 w2 in
-  istore_invariant_disjoint e' f' (fst m0) (fst m1);
+      (p0 `star` p1 `star` hogs_invariant (GS.union e f) (fst m)) m)) =
+  let e' = gs_diff e (hogs_dom (fst m1)) in
+  let _ : squash ((p0 `star` hogs_invariant e' (fst m0)) m0) =
+    let (w1, w2) = star_elim p0 (hogs_invariant e (fst m0)) m0 in
+    hogs_invariant_mono e e' (fst m0) w2;
+    star_intro p0 (hogs_invariant e' (fst m0)) m0 w1 w2 in
+  let f' = gs_diff f (hogs_dom (fst m0)) in
+  let _ : squash ((p1 `star` hogs_invariant f' (fst m1)) m1) =
+    let (w1, w2) = star_elim p1 (hogs_invariant f (fst m1)) m1 in
+    hogs_invariant_mono f f' (fst m1) w2;
+    star_intro p1 (hogs_invariant f' (fst m1)) m1 w1 w2 in
+  hogs_invariant_disjoint e' f' (fst m0) (fst m1);
   let g = GS.union e' f' in
   let m: world = join_worlds m0 m1 in
   star_intro
-    (p0 `star` istore_invariant e' (fst m0)) (p1 `star` istore_invariant f' (fst m1))
+    (p0 `star` hogs_invariant e' (fst m0)) (p1 `star` hogs_invariant f' (fst m1))
     m m0 m1;
   let _ : squash (
-    (p0 `star` istore_invariant e' (fst m0)) `star` (p1 `star` istore_invariant f' (fst m1)) ==
-    (p0 `star` p1) `star` (istore_invariant (GS.union e' f') (fst m))
+    (p0 `star` hogs_invariant e' (fst m0)) `star` (p1 `star` hogs_invariant f' (fst m1)) ==
+    (p0 `star` p1) `star` (hogs_invariant (GS.union e' f') (fst m))
   ) = sep_laws () in
-  let (w1, w2) = star_elim (p0 `star` p1) (istore_invariant (GS.union e' f') (fst m)) m in
-  istore_invariant_mono (GS.union e' f') (GS.union e f) (fst m) w2;
-  star_intro (p0 `star` p1) (istore_invariant (GS.union e f) (fst m)) m w1 w2
+  let (w1, w2) = star_elim (p0 `star` p1) (hogs_invariant (GS.union e' f') (fst m)) m in
+  hogs_invariant_mono (GS.union e' f') (GS.union e f) (fst m) w2;
+  star_intro (p0 `star` p1) (hogs_invariant (GS.union e f) (fst m)) m w1 w2
 
 let max x y = if x > y then x else y
 
-let istore_single n (a: iref) (p: slprop) : okay_istore =
-  let is = mk_istore n fun b -> if reveal a = reveal b then Inv p else None in
+let hogs_single n (a: iref) (p: slprop) : okay_hogs =
+  let is = mk_hogs n fun b -> if reveal a = reveal b then Inv p else None in
   assert fresh_addr is (a + 1);
   is
 
-let rec istore_single_invariant_ n a p f : squash (istore_invariant_ (single a) (istore_single n a p) f == emp) =
+let rec hogs_single_invariant_ n a p f : squash (hogs_invariant_ (single a) (hogs_single n a p) f == emp) =
   if reveal f = 0 then
     ()
   else
-    istore_single_invariant_ n a p (f - 1)
+    hogs_single_invariant_ n a p (f - 1)
 
-let istore_single_invariant n a p : Lemma (istore_invariant (single a) (istore_single n a p) == emp) =
-  istore_single_invariant_ n a p (some_fresh_addr (istore_single n a p))
+let hogs_single_invariant n a p : Lemma (hogs_invariant (single a) (hogs_single n a p) == emp) =
+  hogs_single_invariant_ n a p (some_fresh_addr (hogs_single n a p))
 
-let fresh_inv (p: slprop) (is: okay_istore) (a: iref { None? (read_istore is a) }) :
-    is':okay_istore {
-      disjoint_istore is is' /\
+let fresh_inv (p: slprop) (is: okay_hogs) (a: iref { None? (read_hogs is a) }) :
+    is':okay_hogs {
+      disjoint_hogs is is' /\
       inv_prop a p is' /\
-      istore_invariant (single a) is' == emp /\
-      GS.disjoint (istore_dom is) (istore_dom is')
+      hogs_invariant (single a) is' == emp /\
+      GS.disjoint (hogs_dom is) (hogs_dom is')
     } =
-  let is' = istore_single (level_istore is) a p in
-  istore_single_invariant (level_istore is) a p;
+  let is' = hogs_single (level_hogs is) a p in
+  hogs_single_invariant (level_hogs is) a p;
   is'
 
 let dup_inv_equiv i p : Lemma (inv i p == (inv i p `star` inv i p)) =
